translation/FiatRulesEq.v
@@ -1,0 +1,198 @@
+Set Implicit Arguments.
+From fiat2 Require Import Language TypeSystem TypeSound Value.
+
+Require Import coqutil.Map.Interface coqutil.Datatypes.dlist.
+From Utils Require Import Utils.
+
+From Pyrosome Require Import Theory.WfCutElim Theory.Core Elab.Elab Tools.Matches Lang.SimpleVSubst Lang.SimpleVSTLC.
+From Pyrosome Require Import Lang.FiatTest.
+Import Core.Notations.
+Import coqutil.Datatypes.Result Result.List Result.ResultMonadNotations.
+
+Require Import coqutil.Word.Interface coqutil.Word.Properties.
+
+Require Stdlib.derive.Derive.
+Require Import Datatypes.String Lists.List.
+Open Scope string.
+Import ListNotations.
+Open Scope list.
+
+Require Import Stdlib.FSets.FMapInterface.
+Require Import Stdlib.ZArith.ZArith.
+From Stdlib Require Import Psatz.
+
+Require coqutil.Map.SortedListString.
+Require Import Translator MapUtils Tactics.
+Import SimpleVSubst.
+
+Section WithMap.
+  Context {locals: forall T, map.map string T} 
+  {locals_ok: forall T, map.ok (locals T)}.
+
+  Notation wf_args l :=
+    (wf_args (Model:= core_model l)).
+
+Hint Constructors type_wf: core.
+Hint Resolve conj: core.
+Hint Resolve eq_sort_refl: core.
+
+Lemma ty_sort_wf: wf_sort fiat_rules [] {{s #"ty"}}.
+Proof. eapply wf_sort_by; t''; t'. Qed.
+Lemma list_ty_sort_wf: wf_sort fiat_rules [] {{s #"list_ty"}}.
+Proof. eapply wf_sort_by; t''; t'. Qed.
+Hint Resolve ty_sort_wf list_ty_sort_wf: core.
+
+Local Notation eq_subst l := (eq_subst (Model:= core_model l)).
+Local Notation eq_args l := (eq_args (Model:= core_model l)).
+
+Lemma fiat_wf_lang: wf_lang fiat_rules.
+Proof. unfold fiat_rules. prove_from_known_elabs. Qed.
+Hint Resolve fiat_wf_lang: core.
+Opaque fiat_rules.
+
+Lemma fiat_rule_sort_eq name c s1 s2
+  : ~In (name, sort_eq_rule c s1 s2) fiat_rules.
+Proof.
+  vm_compute; intuition auto.
+  all: repeat match goal with H : _ = _ |- _ => safe_invert H end.
+Qed.
+
+Lemma ty_eq_sort:
+  forall t c (Heq: eq_sort fiat_rules c t {{s #"ty"}}), 
+  t = {{s #"ty"}}.
+Proof.
+  enough (forall t t' c (Heq: eq_sort fiat_rules c t t'), 
+  t = {{s #"ty"}} <-> t' = {{s #"ty"}}) by (intros; eapply H; eauto).
+
+  intros t t' c Heq.
+  induction Heq; eauto; try easy.
+  - eapply fiat_rule_sort_eq in H; inj_all.
+  - destruct t1', t2'.
+    induction l; induction l0; compute in *; apply conj; intros; inj_all.
+  - intuition.
+Qed.
+
+Lemma list_ty_eq_sort:
+  forall t c (Heq: eq_sort fiat_rules c t {{s #"list_ty"}}), 
+  t = {{s #"list_ty"}}.
+Proof.
+  enough (forall t t' c (Heq: eq_sort fiat_rules c t t'), 
+  t = {{s #"list_ty"}} <-> t' = {{s #"list_ty"}}) by (intros; eapply H; eauto).
+
+  intros t t' c Heq.
+  induction Heq; eauto; try easy.
+  - eapply fiat_rule_sort_eq in H; inj_all.
+  - destruct t1', t2'.
+    induction l; induction l0; compute in *; apply conj; intros; inj_all.
+  - intuition.
+Qed.
+
+(*
+Lemma fiat_rule_ty_term_eq name c e1 e2
+  : ~In (name, term_eq_rule c e1 e2 {{s #"ty"}}) fiat_rules.
+Proof.
+  unfold not; intros.
+  repeat (destruct H; equality).
+Qed.
+
+Lemma fiat_rule_list_ty_term_eq name c e1 e2
+  : ~In (name, term_eq_rule c e1 e2 {{s #"list_ty"}}) fiat_rules.
+Proof.
+  unfold not; intros.
+  repeat (destruct H; equality).
+Qed.
+ *)
+
+Lemma ty_eq_term t e1 e2:
+    eq_term fiat_rules [] t e1 e2 ->
+    (t = scon "ty" [] \/ t = scon "list_ty" []) ->
+    e1 = e2.
+Proof.
+  intros H.
+  pattern e2; pattern e1; pattern t; revert t e1 e2 H.
+  apply CutFreeInd.term_cut_ind; try typeclasses eauto; auto.
+  1: apply wf_ctx_nil.
+  all: intros; subst; try now intuition congruence.
+  - destruct H2;
+    repeat (destruct H; equality).
+  - destruct H2.
+    all: destruct t; cbn in H2; inversions.
+    all: destruct l; cbn in H3; inversions; try tauto.
+    all: repeat (destruct H; equality); inj_all.
+    all: repeat lazymatch goal with
+           | H : eq_args _ _ _ _ _ |- _ => safe_invert H
+          | H : (?a = ?b \/ ?a = ?c -> _) |- _ => assert (a=b \/ a=c) by eauto; inj_all
+                         end; auto; repeat f_equal.
+  - destruct H2; inj_all.
+    + eapply ty_eq_sort in H; inj_all.
+    + eapply list_ty_eq_sort in H; inj_all.
+Qed.
+
+Lemma fiat_rule_ext s s0 s1 s2 args t:
+  In ("ext", term_rule [(s, s0); (s1, s2)] args t) fiat_rules ->
+  s0 = {{s #"ty"}} /\ s2 = {{s #"env"}}.
+Proof.
+  intros. repeat (destruct H; equality).
+Qed.
+
+Lemma env_eq_sort:
+  forall t c (Heq: eq_sort fiat_rules c t {{s #"env"}}),
+  t = {{s #"env"}}.
+Proof.
+  enough (forall t t' c (Heq: eq_sort fiat_rules c t t'), 
+  t = scon "env" [] <-> t' = scon "env" []) by (intros; eapply H; eauto).
+  intros t t' c Heq.
+  induction Heq; eauto; try easy.
+  - eapply fiat_rule_sort_eq in H; inj_all.
+  - destruct t1', t2'.
+    induction l; induction l0; compute in *; apply conj; intros; inj_all.
+  - intuition.
+Qed.
+
+Lemma env_eq_term t e1 e2: 
+    eq_term fiat_rules [] t e1 e2 ->
+    t = scon "env" [] ->
+    e1 = e2.
+Proof.
+  intros H.
+  pattern e2; pattern e1; pattern t; revert t e1 e2 H.
+  apply CutFreeInd.term_cut_ind; try typeclasses eauto; auto.
+  1: apply wf_ctx_nil.
+  all: intros; subst; try now intuition congruence.
+  - repeat (destruct H; equality).
+  - destruct t; destruct l; inj_all; inversions.
+    repeat (destruct H; equality); inj_all.
+    repeat lazymatch goal with
+           | H : eq_args _ _ _ _ _ |- _ => safe_invert H
+                         end; auto; repeat f_equal.
+                         eapply ty_eq_term in H11; eauto; inj_all.
+  - destruct t; destruct l; inj_all; inversions.
+    all: eapply env_eq_sort in H; inversions; inj_all.
+Qed.
+
+Lemma eq_sort_trivial_cut_helper: 
+    (forall t t0, eq_sort fiat_rules [] t t0 -> t = t0) /\ 
+    (forall s t t0, eq_term fiat_rules [] s t t0 -> True) /\ 
+    (forall c0 s s0, eq_subst fiat_rules [] c0 s s0 -> True) /\ 
+    (forall c0 s s0, eq_args fiat_rules [] c0 s s0 -> True).
+Proof. 
+  apply CutFreeInd.cut_ind; try typeclasses eauto; eauto; intros; inj_all.
+  - constructor.
+  - eapply fiat_rule_sort_eq in H; tauto.
+  - repeat (destruct H; equality).
+    all: try solve [inversion H0; inj_all].
+    all: repeat lazymatch goal with
+           | H : eq_args _ _ _ _ _ |- _ => safe_invert H
+                         end; auto; cbn in *.
+         all: repeat f_equal. 
+         all: try solve [eapply ty_eq_term; eauto].
+         all: try solve [eapply env_eq_term; eauto].
+Qed.
+
+Lemma eq_sort_trivial s1 s2: 
+    eq_sort fiat_rules [] s1 s2 -> s1 = s2.
+Proof.
+  intros; eapply eq_sort_trivial_cut_helper; eauto.
+Qed.
+
+End WithMap.
