translation/PyroToFiatSound.v
@@ -4,201 +4,121 @@ From fiat2 Require Import Language TypeSystem TypeSound Value.
 Require Import coqutil.Map.Interface coqutil.Datatypes.dlist.
 From Utils Require Import Utils.
 
-From Pyrosome Require Import Theory.WfCutElim Theory.Core Elab.Elab Tools.Matches Lang.SimpleVSubst Lang.SimpleVSTLC.
+From Pyrosome Require Import Theory.WfCutElim Theory.Core.
 From Pyrosome Require Import Lang.FiatTest.
 Import Core.Notations.
 Import coqutil.Datatypes.Result Result.List Result.ResultMonadNotations.
 
 Require Import coqutil.Word.Interface coqutil.Word.Properties.
 
-Require Stdlib.derive.Derive.
 Require Import Datatypes.String Lists.List.
 Open Scope string.
 Import ListNotations.
 Open Scope list.
 
 Require Import Stdlib.FSets.FMapInterface.
-Require Import Stdlib.ZArith.ZArith.
-From Stdlib Require Import Psatz.
 
-Require coqutil.Map.SortedListString.
-Require Import Translator MapUtils Tactics.
+Require Import Translator MapUtils Tactics FiatRulesEq.
 Import SimpleVSubst.
+
+Require Import Psatz.
 
 Section WithMap.
   Context {locals: forall T, map.map string T} 
 {locals_ok: forall T, map.ok (locals T)}.
 
-  Print wf_args.
+  Opaque fiat_rules.
+
   Notation wf_args l :=
     (wf_args (Model:= core_model l)).
 
-Definition pyro_wf_fiat_ty (e:term) (t:sort) :=
-  (t = (scon "ty" []) ->
-  forall ft, Success ft = ty_pyro_to_fiat e ->
-  type_wf ft) /\
-  (t = (scon "list_ty" []) -> 
-  forall tl, Success tl = list_ty_pyro_to_fiat e ->
-  Forall type_wf (map snd tl)).
-
 Hint Constructors type_wf: core.
 Hint Resolve conj: core.
-Hint Resolve eq_sort_refl: core.
 
-Search wf_sort.
-Lemma ty_sort_wf: wf_sort fiat_rules [] (scon "ty" []).
-Proof. eapply wf_sort_by; t''; t'. Qed.
-Lemma list_ty_sort_wf: wf_sort fiat_rules [] (scon "list_ty" []).
-Proof. eapply wf_sort_by; t''; t'. Qed.
 Hint Resolve ty_sort_wf list_ty_sort_wf: core.
 
-Check wf_term_cut_ind.
-Opaque fiat_rules.
+Hint Resolve eq_sort_trivial: core.
 
-Lemma ty_sort_eq:
-  forall t c (Heq: eq_sort fiat_rules c t {{s #"ty"}}), 
-  t = {{s #"ty"}}.
-Proof.
-  enough (forall t t' c (Heq: eq_sort fiat_rules c t t'), 
-  t = {{s #"ty"}} <-> t' = {{s #"ty"}}) by (intros; eapply H; eauto).
-
-  intros t t' c Heq.
-  induction Heq; eauto; try easy.
-  - repeat (destruct H; equality).
-  - destruct t1', t2'.
-    induction l; induction l0; compute in *; apply conj; intros; inj_all.
-  - intuition.
-Qed.
-
-Definition pyro_ty_destruct (e:term) (t:sort) :=
-  (t = {{s #"ty"}} ->
-  e = {{e #"nat"}} \/
-  e = {{e #"bool"}} \/
-  e = {{e #"comparison"}} \/
-  (exists l, e = {{e #"list" {l} }} /\ wf_term fiat_rules [] l {{s #"ty"}}) \/
-  (exists l, e = {{e #"Trecord" {l} }} /\ wf_term fiat_rules [] l {{s #"list_ty"}})).
-
-Lemma ty_sort_destruct:
+(*
+Lemma ty_destruct:
   forall e t,
   wf_term fiat_rules [] e t ->
-  pyro_ty_destruct e t.
+  (fun e t => 
+    (t = {{s #"ty"}} ->
+    e = {{e #"nat"}} \/
+    e = {{e #"bool"}} \/
+    e = {{e #"comparison"}} \/
+    (exists l, e = {{e #"list" {l} }} /\ wf_term fiat_rules [] l {{s #"ty"}}) \/
+    (exists l, e = {{e #"Trecord" {l} }} /\ wf_term fiat_rules [] l {{s #"list_ty"}}))) 
+  e t.
 Proof.
-  apply wf_term_cut_ind; intros;
-  unfold pyro_ty_destruct in *; inj_all.
+  apply wf_term_cut_ind; intros; inj_all.
   + intros. repeat (destruct H; equality).
     all: repeat (destruct s; inj_all).
     - inversion H0; inj_all.
       repeat right; eexists; eauto.
     - inversion H0; inj_all.
       do 3 right; left. eexists; eauto.
-  + intros. inj_all. eapply ty_sort_eq in H1; inj_all.
-Qed.
-
-Lemma list_ty_sort_eq:
-  forall t c (Heq: eq_sort fiat_rules c t {{s #"list_ty"}}),
-  t = {{s #"list_ty"}}.
-Proof.
-  enough (forall t t' c (Heq: eq_sort fiat_rules c t t'), 
-  t = scon "list_ty" [] <-> t' = scon "list_ty" []) by (intros; eapply H; eauto).
-  intros t t' c Heq.
-  induction Heq; eauto; try easy.
-  - repeat (destruct H; equality).
-  - destruct t1', t2'.
-    induction l; induction l0; compute in *; apply conj; intros; inj_all.
-  - intuition.
-Qed.
-
-Hint Resolve ty_sort_eq list_ty_sort_eq: core.
+  + intros. inj_all. eapply ty_eq_sort in H1; inj_all.
+   Qed. *)
 
 Theorem ty_pyro_to_fiat_wf:
   forall (Gp:term) (t:sort)
   (Hpwf: wf_term fiat_rules [] Gp t),
-  (pyro_wf_fiat_ty Gp t).
+  (fun e t =>
+    (t = {{s #"ty"}} ->
+    forall ft, Success ft = ty_pyro_to_fiat e -> type_wf ft) /\
+    (t = {{s #"list_ty"}} -> 
+    forall tl, Success tl = list_ty_pyro_to_fiat e ->
+    Forall type_wf tl)
+  ) Gp t.
 Proof.
-  unfold pyro_wf_fiat_ty.
-  apply wf_term_cut_ind; intros; cycle 1.
-  - inj_all.
-  - apply conj; intros; inj_all; eauto.
-  - apply conj; intros.
+  apply wf_term_cut_ind; intros; intuition; try solve [inj_all].
     * repeat (destruct H; equality).
       all: inj_all.
-        enough (type_wf (TRecord a) /\ Forall (fun p => forall q, of_nat q = fst p -> length a > q) a) by intuition.
-        clear H H0 H1.
-        generalize dependent t.
-        induction a; intros; destruct t; try solve [repeat constructor; eauto]; invert_cons.
-        specialize IHa with t0; inj_all.
-        inversion H; inj_all.
-        pose proof Forall_map_fst as Hfst.
-        specialize Hfst with (P:=(fun x => forall q, of_nat q = x -> length a1 > q)); simpl in Hfst.
-        apply Hfst in H0.
-
-        apply conj; constructor; invert_cons; try constructor; eauto.
-        + unfold "~"; intros.
-          From Stdlib Require Import Psatz.
-          eapply Forall_In in H2; try eapply H0; inj_all.
-          specialize H2 with (length a1); inj_all; lia.
-        + admit.
-        + apply of_nat_inj in H2; inj_all.
-          admit.
-        + apply Hfst in H0.
-          eapply Forall_impl; try eapply H0; eauto.
-    * inj_all;
-      repeat (destruct H; equality); inj_all.
-Admitted.
+      inversion H0; inj_all. 
+      clear H1. 
+      pose proof name_list_ty_ok a. constructor; inj_all.
+    * repeat (destruct H; equality).
+      all: inj_all. 
+Qed.
 
 Hint Resolve ty_pyro_to_fiat_wf: core.
-
-Lemma env_sort_eq:
-  forall t c (Heq: eq_sort fiat_rules c t (scon "env" [])), 
-  t = scon "env" [].
-Proof.
-  enough (forall t t' c (Heq: eq_sort fiat_rules c t t'), 
-  t = scon "env" [] <-> t' = scon "env" []) by (intros; eapply H; eauto).
-  intros t t' c Heq.
-  induction Heq; eauto; try easy.
-  - repeat (destruct H; equality).
-  - destruct t1', t2'.
-    induction l; induction l0; compute in *; apply conj; intros; inj_all.
-  - intuition.
-Qed.
-Hint Resolve env_sort_eq: core.
-
-Definition env_pyro_to_fiat_wf_term  (Gp:term) (t:sort)  :=
-  forall (Genv: list(string*type))
-  (Hs: t = scon "env" [])
-  (Henv: Success Genv = env_pyro_to_fiat Gp),
-  exists fenv, (fenv_wf Genv fenv /\
-  forall t n, map.get fenv (of_nat n) = Some t ->
-  n < length Genv).
 
 Theorem env_pyro_to_fiat_wf:
   forall (Gp:term) (t:sort)
   (Hpwf: wf_term fiat_rules [] Gp t),
-  env_pyro_to_fiat_wf_term Gp t.
+  (fun e t =>
+    forall (Genv: lenv)
+    (Henv: Success Genv = env_pyro_to_fiat e),
+    t = {{s #"env"}} ->
+    exists fenv, (fenv_wf Genv fenv /\
+    forall t n, map.get fenv (of_nat n) = Some t ->
+  n < length Genv)
+  ) Gp t.
+
 Proof.
   apply wf_term_cut_ind;
-  unfold env_pyro_to_fiat_wf_term;
-  intros; intuition; inj_all; eauto.
+  intros; intuition; inj_all.
   - eexists; apply conj; try eapply fenv_wf_nil; intros; map_simpl.
-  - repeat (destruct H; equality).
-    clear H2; specialize H3 with a0; inj_all.
+  - apply fiat_rule_ext in H; inj_all.
+    clear H3. 
     eexists; apply conj; try eapply fenv_wf_cons; intros; eauto; map_simpl.
-      * specialize H2 with (n:=length a0). 
+      * specialize H4 with (n:=length a0). 
         destruct (map.get x (of_nat (length a0))); inj_all.
-        specialize H2 with t; inj_all. lia.
+        specialize H4 with t2; inj_all. lia.
       * eapply ty_pyro_to_fiat_wf in case_match_eqn; eauto.
         inversion H0; eauto.
       * assert (Hneq: n=length a0 \/ n<>length a0) by lia.
         destruct Hneq; inj_all. 
         assert (of_nat (length a0) <> of_nat n). {
         unfold "<>"; intros. 
-        apply of_nat_inj in H5. lia.
+        apply of_nat_inj in H6. lia.
         }
-        map_simpl. apply H2 in H3; lia.
+        map_simpl. apply H4 in H3; lia.
 Qed.
 
 Hint Resolve env_pyro_to_fiat_wf: core.
-
 
 (*
    induction on judgement structure...
@@ -213,7 +133,10 @@ Hint Resolve env_pyro_to_fiat_wf: core.
    free vs bound variables
  *) 
 
-Definition pyro_expr_wf (e:term) (t:sort) :=
+Theorem expr_pyro_to_fiat_wf: 
+  forall (pt:term) (t:sort)
+  (Hpwf: wf_term fiat_rules [] pt t),
+  (fun e t =>
   forall A Gp, 
   t = scon "val" [A;Gp] ->
   forall fe, Success fe = expr_pyro_to_fiat e ->
@@ -221,92 +144,22 @@ Definition pyro_expr_wf (e:term) (t:sort) :=
   Success ft = ty_pyro_to_fiat A ->
   Success Genv = env_pyro_to_fiat Gp ->
   fenv_wf Genv fenv ->
-  type_of map.empty fenv fe ft.
-
-Lemma val_sort_eq:
-  forall t A Gp (Heq: eq_sort fiat_rules [] t (scon "val" [A;Gp]))
-  (Ha: wf_term fiat_rules [] A (scon "ty" []))
-  (HG: wf_term fiat_rules [] Gp (scon "env" [])),
-  exists A' Gp',
-  t = scon "val" [A';Gp'] /\
-  eq_term fiat_rules [] (scon "ty" []) A A' /\ 
-  eq_term fiat_rules [] (scon "env" []) Gp Gp'.
-Proof.
-  intros. 
-  induction Heq; intros; inj_all; eauto.
-  - repeat (destruct H; equality).
-  - induction s1; destruct s2; inversion H; invert_cons.
-    + rewrite sort_subst_nil. 
-      repeat eexists. ; try rewrite term_subst_nil; auto.
-    + clear IHHeq.
-      Search term_subst.
-      inversion Ha; inj_all.
-Unset Printing Notations.
-    Search apply_subst.
-    
-
-
-(*
-Lemma val_sort_eq:
-  forall t c A Gp (Heq: eq_sort fiat_rules c t (scon "val" [A;Gp]))
-  (Ha: wf_term fiat_rules c A (scon "ty" []))
-  (HG: wf_term fiat_rules c Gp (scon "env" [])),
-  t = scon "val" [A;Gp].
-Proof.
-  intros.
-  inj_all.
-  pose proof ty_sort_eq.
-
-
-  enough (forall t t' c (Heq: eq_sort fiat_rules c t t') A Gp,
-  (*(Ha: wf_term fiat_rules c A (scon "ty" []))
-     (HG: wf_term fiat_rules c Gp (scon "env" [])),*)
-  t = scon "val" [A;Gp] <-> t' = scon "val" [A;Gp]) by (intros; eapply H; eauto).
-  intros t t' c Heq.
-  induction Heq; intros; eauto.
-  - intros; subst.
-    repeat (destruct H; equality).
-  - intros; subst.
-    destruct t1', t2'. 
-    apply conj; intros; inversion H1; inj_all.
-    + do 3 (destruct l; inj_all).
-      inversion H4; inj_all.
-      specialize IHHeq with t t0; destruct IHHeq; inj_all.
-      inversion H1; inj_all.
-      enough (term_subst s2 t0 = term_subst s1 t0 /\ term_subst s2 t = term_subst s1 t). {
-        inj_all; f_equal; f_equal; eauto; f_equal; eauto.
-      }
-      f_equal; cbn.
-      
-      Search eq_subst.
-      repeat f_equal.
-
-Qed.
- *)
-
-Theorem expr_pyro_to_fiat_wf: 
-  forall (pt:term) (t:sort)
-  (Hpwf: wf_term fiat_rules [] pt t),
-  (pyro_expr_wf pt t).
+  type_of map.empty fenv fe ft
+  ) pt t.
 Proof.
   apply wf_term_cut_ind;
-  unfold pyro_expr_wf;
-  intros; intuition.
+  intros; intuition; cycle 1.
+  - apply eq_sort_trivial in H1; inj_all.
+    edestruct H0; eauto.
   - repeat (destruct H; equality).
-    all: inj_all.
-    all: cbn in *.
-    all: inversion H2; inj_all.
+    all: inversions.
+    all: do_both; cbn in *.
     all: try solve [repeat econstructor; eauto].
-    + specialize H1 with (con "list" [t1]) Gp a0 (TList a1) Genv fenv; inj_all.
+    + specialize H2 with (con "list" [t1]) t2 a1 (TList a) Genv fenv; inj_all.
       repeat econstructor; eauto.
     + inversion H0; clear H0; inj_all.
-      repeat econstructor; eapply ty_pyro_to_fiat_wf; eauto.
-  - inj_all.
-    inversion H1; inj_all.
-    + repeat (destruct H2; equality).
-    + 
-    
+      eapply ty_pyro_to_fiat_wf in H10; inj_all.
+      repeat econstructor; eauto.
 Qed.
-
 
 End WithMap.
